Add close constructor

theories/autosubst/CCAST.sig
@@ -6,6 +6,8 @@ cmode : Type
 
 cterm(cvar) : Type
 
+close : (bind cterm in cterm) -> cterm
+
 cSort : cmode -> level -> cterm
 
 cPi : cmode -> cterm -> (bind cterm in cterm) -> cterm
