theories/autosubst/CCAST.v
@@ -7,6 +7,7 @@ Module Core.
 
 Inductive cterm : Type :=
   | cvar : nat -> cterm
+  | close : cterm -> cterm
   | cSort : cmode -> level -> cterm
   | cPi : cmode -> cterm -> cterm -> cterm
   | clam : cmode -> cterm -> cterm -> cterm
@@ -22,6 +23,12 @@ Inductive cterm : Type :=
   | ctyerr : cterm
   | cEl : cterm -> cterm
   | cErr : cterm -> cterm.
+
+Lemma congr_close {s0 : cterm} {t0 : cterm} (H0 : s0 = t0) :
+  close s0 = close t0.
+Proof.
+exact (eq_trans eq_refl (ap (fun x => close x) H0)).
+Qed.
 
 Lemma congr_cSort {s0 : cmode} {s1 : level} {t0 : cmode} {t1 : level}
   (H0 : s0 = t0) (H1 : s1 = t1) : cSort s0 s1 = cSort t0 t1.
@@ -125,6 +132,7 @@ Defined.
 Fixpoint ren_cterm (xi_cterm : nat -> nat) (s : cterm) {struct s} : cterm :=
   match s with
   | cvar s0 => cvar (xi_cterm s0)
+  | close s0 => close (ren_cterm (upRen_cterm_cterm xi_cterm) s0)
   | cSort s0 s1 => cSort s0 s1
   | cPi s0 s1 s2 =>
       cPi s0 (ren_cterm xi_cterm s1)
@@ -156,6 +164,7 @@ Fixpoint subst_cterm (sigma_cterm : nat -> cterm) (s : cterm) {struct s} :
 cterm :=
   match s with
   | cvar s0 => sigma_cterm s0
+  | close s0 => close (subst_cterm (up_cterm_cterm sigma_cterm) s0)
   | cSort s0 s1 => cSort s0 s1
   | cPi s0 s1 s2 =>
       cPi s0 (subst_cterm sigma_cterm s1)
@@ -196,6 +205,10 @@ Fixpoint idSubst_cterm (sigma_cterm : nat -> cterm)
 subst_cterm sigma_cterm s = s :=
   match s with
   | cvar s0 => Eq_cterm s0
+  | close s0 =>
+      congr_close
+        (idSubst_cterm (up_cterm_cterm sigma_cterm)
+           (upId_cterm_cterm _ Eq_cterm) s0)
   | cSort s0 s1 => congr_cSort (eq_refl s0) (eq_refl s1)
   | cPi s0 s1 s2 =>
       congr_cPi (eq_refl s0) (idSubst_cterm sigma_cterm Eq_cterm s1)
@@ -240,6 +253,11 @@ Fixpoint extRen_cterm (xi_cterm : nat -> nat) (zeta_cterm : nat -> nat)
 ren_cterm xi_cterm s = ren_cterm zeta_cterm s :=
   match s with
   | cvar s0 => ap (cvar) (Eq_cterm s0)
+  | close s0 =>
+      congr_close
+        (extRen_cterm (upRen_cterm_cterm xi_cterm)
+           (upRen_cterm_cterm zeta_cterm) (upExtRen_cterm_cterm _ _ Eq_cterm)
+           s0)
   | cSort s0 s1 => congr_cSort (eq_refl s0) (eq_refl s1)
   | cPi s0 s1 s2 =>
       congr_cPi (eq_refl s0) (extRen_cterm xi_cterm zeta_cterm Eq_cterm s1)
@@ -288,6 +306,10 @@ Fixpoint ext_cterm (sigma_cterm : nat -> cterm) (tau_cterm : nat -> cterm)
 subst_cterm sigma_cterm s = subst_cterm tau_cterm s :=
   match s with
   | cvar s0 => Eq_cterm s0
+  | close s0 =>
+      congr_close
+        (ext_cterm (up_cterm_cterm sigma_cterm) (up_cterm_cterm tau_cterm)
+           (upExt_cterm_cterm _ _ Eq_cterm) s0)
   | cSort s0 s1 => congr_cSort (eq_refl s0) (eq_refl s1)
   | cPi s0 s1 s2 =>
       congr_cPi (eq_refl s0) (ext_cterm sigma_cterm tau_cterm Eq_cterm s1)
@@ -334,6 +356,11 @@ Fixpoint compRenRen_cterm (xi_cterm : nat -> nat) (zeta_cterm : nat -> nat)
 ren_cterm zeta_cterm (ren_cterm xi_cterm s) = ren_cterm rho_cterm s :=
   match s with
   | cvar s0 => ap (cvar) (Eq_cterm s0)
+  | close s0 =>
+      congr_close
+        (compRenRen_cterm (upRen_cterm_cterm xi_cterm)
+           (upRen_cterm_cterm zeta_cterm) (upRen_cterm_cterm rho_cterm)
+           (up_ren_ren _ _ _ Eq_cterm) s0)
   | cSort s0 s1 => congr_cSort (eq_refl s0) (eq_refl s1)
   | cPi s0 s1 s2 =>
       congr_cPi (eq_refl s0)
@@ -391,6 +418,11 @@ Fixpoint compRenSubst_cterm (xi_cterm : nat -> nat)
 subst_cterm tau_cterm (ren_cterm xi_cterm s) = subst_cterm theta_cterm s :=
   match s with
   | cvar s0 => Eq_cterm s0
+  | close s0 =>
+      congr_close
+        (compRenSubst_cterm (upRen_cterm_cterm xi_cterm)
+           (up_cterm_cterm tau_cterm) (up_cterm_cterm theta_cterm)
+           (up_ren_subst_cterm_cterm _ _ _ Eq_cterm) s0)
   | cSort s0 s1 => congr_cSort (eq_refl s0) (eq_refl s1)
   | cPi s0 s1 s2 =>
       congr_cPi (eq_refl s0)
@@ -462,6 +494,11 @@ ren_cterm zeta_cterm (subst_cterm sigma_cterm s) = subst_cterm theta_cterm s
 :=
   match s with
   | cvar s0 => Eq_cterm s0
+  | close s0 =>
+      congr_close
+        (compSubstRen_cterm (up_cterm_cterm sigma_cterm)
+           (upRen_cterm_cterm zeta_cterm) (up_cterm_cterm theta_cterm)
+           (up_subst_ren_cterm_cterm _ _ _ Eq_cterm) s0)
   | cSort s0 s1 => congr_cSort (eq_refl s0) (eq_refl s1)
   | cPi s0 s1 s2 =>
       congr_cPi (eq_refl s0)
@@ -535,6 +572,11 @@ subst_cterm tau_cterm (subst_cterm sigma_cterm s) = subst_cterm theta_cterm s
 :=
   match s with
   | cvar s0 => Eq_cterm s0
+  | close s0 =>
+      congr_close
+        (compSubstSubst_cterm (up_cterm_cterm sigma_cterm)
+           (up_cterm_cterm tau_cterm) (up_cterm_cterm theta_cterm)
+           (up_subst_subst_cterm_cterm _ _ _ Eq_cterm) s0)
   | cSort s0 s1 => congr_cSort (eq_refl s0) (eq_refl s1)
   | cPi s0 s1 s2 =>
       congr_cPi (eq_refl s0)
@@ -662,6 +704,11 @@ Fixpoint rinst_inst_cterm (xi_cterm : nat -> nat)
 {struct s} : ren_cterm xi_cterm s = subst_cterm sigma_cterm s :=
   match s with
   | cvar s0 => Eq_cterm s0
+  | close s0 =>
+      congr_close
+        (rinst_inst_cterm (upRen_cterm_cterm xi_cterm)
+           (up_cterm_cterm sigma_cterm)
+           (rinstInst_up_cterm_cterm _ _ Eq_cterm) s0)
   | cSort s0 s1 => congr_cSort (eq_refl s0) (eq_refl s1)
   | cPi s0 s1 s2 =>
       congr_cPi (eq_refl s0)
@@ -896,6 +943,7 @@ Defined.
 Fixpoint allfv_cterm (p_cterm : nat -> Prop) (s : cterm) {struct s} : Prop :=
   match s with
   | cvar s0 => p_cterm s0
+  | close s0 => and (allfv_cterm (upAllfv_cterm_cterm p_cterm) s0) True
   | cSort s0 s1 => and True (and True True)
   | cPi s0 s1 s2 =>
       and True
@@ -937,6 +985,10 @@ Fixpoint allfvTriv_cterm (p_cterm : nat -> Prop)
 allfv_cterm p_cterm s :=
   match s with
   | cvar s0 => H_cterm s0
+  | close s0 =>
+      conj
+        (allfvTriv_cterm (upAllfv_cterm_cterm p_cterm)
+           (upAllfvTriv_cterm_cterm H_cterm) s0) I
   | cSort s0 s1 => conj I (conj I I)
   | cPi s0 s1 s2 =>
       conj I
@@ -986,6 +1038,14 @@ Fixpoint allfvImpl_cterm (p_cterm : nat -> Prop) (q_cterm : nat -> Prop)
 allfv_cterm p_cterm s -> allfv_cterm q_cterm s :=
   match s with
   | cvar s0 => fun HP => H_cterm s0 HP
+  | close s0 =>
+      fun HP =>
+      conj
+        (allfvImpl_cterm (upAllfv_cterm_cterm p_cterm)
+           (upAllfv_cterm_cterm q_cterm) (upAllfvImpl_cterm_cterm H_cterm) s0
+           match HP with
+           | conj HP _ => HP
+           end) I
   | cSort s0 s1 => fun HP => conj I (conj I I)
   | cPi s0 s1 s2 =>
       fun HP =>
@@ -1119,6 +1179,15 @@ allfv_cterm p_cterm (ren_cterm xi_cterm s) ->
 allfv_cterm (funcomp p_cterm xi_cterm) s :=
   match s with
   | cvar s0 => fun H => H
+  | close s0 =>
+      fun H =>
+      conj
+        (allfvImpl_cterm _ _ (upAllfvRenL_cterm_cterm p_cterm xi_cterm) s0
+           (allfvRenL_cterm (upAllfv_cterm_cterm p_cterm)
+              (upRen_cterm_cterm xi_cterm) s0
+              match H with
+              | conj H _ => H
+              end)) I
   | cSort s0 s1 => fun H => conj I (conj I I)
   | cPi s0 s1 s2 =>
       fun H =>
@@ -1250,6 +1319,15 @@ allfv_cterm (funcomp p_cterm xi_cterm) s ->
 allfv_cterm p_cterm (ren_cterm xi_cterm s) :=
   match s with
   | cvar s0 => fun H => H
+  | close s0 =>
+      fun H =>
+      conj
+        (allfvRenR_cterm (upAllfv_cterm_cterm p_cterm)
+           (upRen_cterm_cterm xi_cterm) s0
+           (allfvImpl_cterm _ _ (upAllfvRenR_cterm_cterm p_cterm xi_cterm) s0
+              match H with
+              | conj H _ => H
+              end)) I
   | cSort s0 s1 => fun H => conj I (conj I I)
   | cPi s0 s1 s2 =>
       fun H =>
